theories/examples/future_fibonacci.v
@@ -87,7 +87,7 @@ Section future_G.
       rewrite Nat2Z.id. iSteps.
     }
 
-    wp_apply+ (pool_kill_spec with "Hpool_model").
+    wp_apply+ (pool_close_spec with "Hpool_model").
     iSteps.
   Qed.
 End future_G.
