theories/examples/pool_quicksort.v
@@ -333,7 +333,7 @@ Section pool_G.
     }
 
     iApply wp_fupd.
-    wp_apply+ (pool_kill_spec with "[$Hpool_model]") as "#Hpool_finished".
+    wp_apply+ (pool_close_spec with "[$Hpool_model]") as "#Hpool_finished".
     iMod (pool_consumer_finished with "Hpool_consumer Hpool_finished") as "(%xs' & % & % & Harr)".
     iSteps.
   Qed.
