theories/examples/vertex_fibonacci.v
@@ -177,7 +177,7 @@ Section vertex_fibonacci_G.
       iSteps.
     }
 
-    wp_apply+ (pool_kill_spec with "Hpool_model").
+    wp_apply+ (pool_close_spec with "Hpool_model").
     iSteps.
   Qed.
 End vertex_fibonacci_G.
