theories/zoo_parabs/ws_hub_std__types.v
@@ -27,7 +27,7 @@ Notation "'waiters'" := (
   in_type "zoo_parabs.ws_hub_std.t" 2
 )(in custom zoo_field
 ).
-Notation "'killed'" := (
+Notation "'num_active'" := (
   in_type "zoo_parabs.ws_hub_std.t" 3
 )(in custom zoo_field
 ).
